Format some errors

src/typechecker/FStar.TypeChecker.Normalize.fst
@@ -3203,6 +3203,13 @@ let comp_to_string env c = GenSym.with_frozen_gensym (fun () ->
   in
   Print.comp_to_string' (DsEnv.set_current_module env.dsenv env.curmodule) c)
 
+let comp_to_doc env c = GenSym.with_frozen_gensym (fun () ->
+  let c =
+    try norm_comp (config [AllowUnboundUniverses] env) [] c
+    with e -> Errors.log_issue c.pos (Errors.Warning_NormalizationFailure, (BU.format1 "Normalization failed with error %s\n" (BU.message_of_exn e))) ; c
+  in
+  Print.comp_to_doc' (DsEnv.set_current_module env.dsenv env.curmodule) c)
+
 let normalize_refinement steps env t0 =
    let t = normalize (steps@[Beta]) env t0 in
    U.flatten_refinement t
